Mathbin/AlgebraicGeometry/FunctionField.lean
@@ -204,7 +204,7 @@ theorem functionField_isFractionRing_of_isAffineOpen [IsIntegral X] (U : Opens X
 -/
 
 instance (x : X.carrier) : IsAffine (X.affineCover.obj x) :=
-  AlgebraicGeometry.SpecIsAffine _
+  AlgebraicGeometry.isAffine_Spec _
 
 instance [h : IsIntegral X] (x : X.carrier) : IsFractionRing (X.Presheaf.stalk x) X.functionField :=
   by
