Mathbin/AlgebraicGeometry/Limits.lean
@@ -46,7 +46,7 @@ instance : HasTerminal Scheme :=
   hasTerminal_of_hasTerminal_of_preservesLimit Scheme.Spec
 
 instance : IsAffine (⊤_ Scheme.{u}) :=
-  isAffineOfIso (PreservesTerminal.iso Scheme.Spec).inv
+  isAffine_of_isIso (PreservesTerminal.iso Scheme.Spec).inv
 
 instance : HasFiniteLimits Scheme :=
   hasFiniteLimits_of_hasTerminal_and_pullbacks
@@ -141,7 +141,7 @@ noncomputable def specPunitIsInitial : IsInitial (Scheme.Spec.obj (op <| CommRin
 
 #print AlgebraicGeometry.isAffine_of_isEmpty /-
 instance (priority := 100) isAffine_of_isEmpty {X : Scheme} [IsEmpty X.carrier] : IsAffine X :=
-  isAffineOfIso
+  isAffine_of_isIso
     (inv (emptyIsInitial.to X) ≫ emptyIsInitial.to (Scheme.Spec.obj (op <| CommRingCat.of PUnit)))
 #align algebraic_geometry.is_affine_of_is_empty AlgebraicGeometry.isAffine_of_isEmpty
 -/
@@ -155,13 +155,13 @@ instance initial_isEmpty : IsEmpty (⊥_ Scheme).carrier :=
 #align algebraic_geometry.initial_is_empty AlgebraicGeometry.initial_isEmpty
 -/
 
-#print AlgebraicGeometry.bot_isAffineOpen /-
-theorem bot_isAffineOpen (X : Scheme) : IsAffineOpen (⊥ : Opens X.carrier) :=
+#print AlgebraicGeometry.isAffineOpen_bot /-
+theorem isAffineOpen_bot (X : Scheme) : IsAffineOpen (⊥ : Opens X.carrier) :=
   by
   convert range_is_affine_open_of_open_immersion (initial.to X)
   ext
   exact (false_iff_iff _).mpr fun x => isEmptyElim (show (⊥_ Scheme).carrier from x.some)
-#align algebraic_geometry.bot_is_affine_open AlgebraicGeometry.bot_isAffineOpen
+#align algebraic_geometry.bot_is_affine_open AlgebraicGeometry.isAffineOpen_bot
 -/
 
 instance : HasStrictInitialObjects Scheme :=
