Mathbin/AlgebraicGeometry/Morphisms/QuasiCompact.lean
@@ -103,7 +103,7 @@ theorem isCompact_open_iff_eq_basicOpen_union {X : Scheme} [IsAffine X] (U : Set
       ∃ s : Set (X.Presheaf.obj (op ⊤)),
         s.Finite ∧ U = ⋃ (i : X.Presheaf.obj (op ⊤)) (h : i ∈ s), X.basicOpen i :=
   (isBasis_basicOpen X).isCompact_open_iff_eq_finite_iUnion _
-    (fun i => ((topIsAffineOpen _).basicOpenIsAffine _).IsCompact) _
+    (fun i => ((isAffineOpen_top _).basicOpen _).IsCompact) _
 #align algebraic_geometry.is_compact_open_iff_eq_basic_open_union AlgebraicGeometry.isCompact_open_iff_eq_basicOpen_union
 -/
 
@@ -225,11 +225,11 @@ theorem QuasiCompact.affine_openCover_tfae {X Y : Scheme.{u}} (f : X ⟶ Y) :
 #align algebraic_geometry.quasi_compact.affine_open_cover_tfae AlgebraicGeometry.QuasiCompact.affine_openCover_tfae
 -/
 
-#print AlgebraicGeometry.QuasiCompact.is_local_at_target /-
-theorem QuasiCompact.is_local_at_target : PropertyIsLocalAtTarget @QuasiCompact :=
+#print AlgebraicGeometry.QuasiCompact.isLocalAtTarget /-
+theorem QuasiCompact.isLocalAtTarget : PropertyIsLocalAtTarget @QuasiCompact :=
   quasiCompact_eq_affineProperty.symm ▸
-    QuasiCompact.affineProperty_isLocal.targetAffineLocallyIsLocal
-#align algebraic_geometry.quasi_compact.is_local_at_target AlgebraicGeometry.QuasiCompact.is_local_at_target
+    QuasiCompact.affineProperty_isLocal.targetAffineLocally_isLocal
+#align algebraic_geometry.quasi_compact.is_local_at_target AlgebraicGeometry.QuasiCompact.isLocalAtTarget
 -/
 
 #print AlgebraicGeometry.QuasiCompact.openCover_tfae /-
@@ -245,7 +245,7 @@ theorem QuasiCompact.openCover_tfae {X Y : Scheme.{u}} (f : X ⟶ Y) :
           QuasiCompact (pullback.snd : pullback f g ⟶ _),
         ∃ (ι : Type u) (U : ι → Opens Y.carrier) (hU : iSup U = ⊤), ∀ i, QuasiCompact (f ∣_ U i)] :=
   quasiCompact_eq_affineProperty.symm ▸
-    QuasiCompact.affineProperty_isLocal.targetAffineLocallyIsLocal.openCover_TFAE f
+    QuasiCompact.affineProperty_isLocal.targetAffineLocally_isLocal.openCover_TFAE f
 #align algebraic_geometry.quasi_compact.open_cover_tfae AlgebraicGeometry.QuasiCompact.openCover_tfae
 -/
 
@@ -275,7 +275,7 @@ theorem QuasiCompact.affine_openCover_iff {X Y : Scheme.{u}} (𝒰 : Scheme.Open
 theorem QuasiCompact.openCover_iff {X Y : Scheme.{u}} (𝒰 : Scheme.OpenCover.{u} Y) (f : X ⟶ Y) :
     QuasiCompact f ↔ ∀ i, QuasiCompact (pullback.snd : pullback f (𝒰.map i) ⟶ _) :=
   quasiCompact_eq_affineProperty.symm ▸
-    QuasiCompact.affineProperty_isLocal.targetAffineLocallyIsLocal.openCover_iff f 𝒰
+    QuasiCompact.affineProperty_isLocal.targetAffineLocally_isLocal.openCover_iff f 𝒰
 #align algebraic_geometry.quasi_compact.open_cover_iff AlgebraicGeometry.QuasiCompact.openCover_iff
 -/
 
